\input{../article_base.tex}

\usepackage{ifthen}

\begin{document}

נגדיר $\Omega = [6]$ עם הסתברות אחידה $\PP$.
נגדיר $X(\omega) = \omega$ ו־$Y(\omega) = \omega$
\[
	Supp X = [6]
	\qquad
	Supp Y = [6]
\]
נגדיר $Z = X + Y$.
\[
	Supp Z = 2 \cdot [6]
\]
עכשיו נגדיר $X$ הטלת קובייה ו־$Y$ הטלת קובייה שנייה. עכשיו $\Omega = {[6]}^2$.
\[
	X((a, b)) = a,
	\qquad
	Y((a, b)) = b,
	\qquad
	Z((a, b)) = a + b
	\qquad
	Supp Z = [12]
\]
נחשב
\[
	\PP(Z = 4) = \PP(\{(1, 3), (3, 1), (2, 2)\}) = \frac{3}{36}
	= \PP(\{\omega \in \Omega \mid Z(\omega) = 4\})
\]

$Supp\ X = Supp\ Y = \{0, \dots, n - 1\}$ וגם $Z = X + Y \mod n$.
\[
	Supp\ Z = Supp\ X = \{0, \dots, n - 1\}
\]
נניח ש־$X, Z$ בלתי־תלויים. נראה ש־$\PP(Y = \omega) = \frac{1}{n}$.
\begin{align*}
	\PP(X = k) \cdot \PP(Z = l)
	& = \PP(X = k, Z = l) \\
	& = \PP(X = k, X + Y \mod n = l) \\
	& = \PP(X = k, X + Y = l + a n) \\
	& = \PP(X = k, X + Y \in \{l, l + n\}) \\
	& = \PP(X = k, k + Y \in \{l, l + n\}) \\
	& = \PP(X = k, Y \in \{l - k, l - k + n\}) \\
	& = \PP(X = k) \PP(Y \in \{l - k, l - k + n\}) \\
\end{align*}
ולכן
\[
	\PP(Z = l) = \PP(Y \in \{l - k, l - k + n\})
\]
נחפש את
\[
	\PP(Y = m)
\]
נקבל $m = l - k$ או $m = l - k + n$.
\[
	\PP(Y = m) = \PP(Z = l)
\]
נכתוב $l = m + k$ או $l = m + k - n$.
\[
	\PP(Y = m) = \PP(Z = m + k)
\]
נגדיר $k = i, j$
אז
\[
	\PP(Y = m) = \PP(Z = m + i) = \PP(Z = m + j)
\]
לדוגמה אם $m = 0$ אז
\[
	\PP(Z = i) = \PP(Z = j)
\]
לכל $0 \le i, j \le n - 1$.
לכן
\[
	\PP(Z = l) = \frac{1}{n}
\]
אז נובע
\[
	\PP(Y = m) = \frac{1}{n}
\]

\end{document}
